Add rewrite to split conjunction; add experiment code for the triangle example

fiat2/src/fiat2/Ex_Family.v
@@ -21,13 +21,13 @@ foreach person in queries do
             check(p.parent = person && q.parent = p.child),
             ret q.child ] in
     foreach child in children do
-        result := mut result ++ "child" ++ "\n"
+        result := mut result ++ child ++ "\n"
     end;
     outputs := mut result :: mut outputs
 end
 *)
 
-Definition prog := (CLetMut (EVar "parents_tbl") "parents" (CForeach (EVar "queries") "person" (CLetMut (EBinop OConcatString (EAtom (AString "Grandchildren of ")) (EBinop OConcatString (EVar "person") (EAtom (AString ":\n")))) "result" (CLet (ESort LikeList (EFlatmap LikeList (ELoc "parents") "p" (EFlatmap LikeList (ELoc "parents") "q" (EIf (EBinop OEq (EAccess (EVar "p") "parent") (EBinop OAnd (EVar "person") (EBinop OEq (EAccess (EVar "q") "parent") (EAccess (EVar "p") "child")))) (EBinop OCons (EAccess (EVar "q") "child") (EAtom (ANil None))) (EAtom (ANil None)))))) "children" (CSeq (CForeach (EVar "children") "child" (CAssign "result" (EBinop OConcatString (ELoc "result") (EBinop OConcatString (EAtom (AString "child")) (EAtom (AString "\n")))))) (CAssign "outputs" (EBinop OCons (ELoc "result") (ELoc "outputs")))))))).
+Definition prog := (CLetMut (EVar "parents_tbl") "parents" (CForeach (EVar "queries") "person" (CLetMut (EBinop OConcatString (EAtom (AString "Grandchildren of ")) (EBinop OConcatString (EVar "person") (EAtom (AString ":\n")))) "result" (CLet (ESort LikeList (EFlatmap LikeList (ELoc "parents") "p" (EFlatmap LikeList (ELoc "parents") "q" (EIf (EBinop OAnd (EBinop OEq (EAccess (EVar "p") "parent") (EVar "person")) (EBinop OEq (EAccess (EVar "q") "parent") (EAccess (EVar "p") "child"))) (EBinop OCons (EAccess (EVar "q") "child") (EAtom (ANil None))) (EAtom (ANil None)))))) "children" (CSeq (CForeach (EVar "children") "child" (CAssign "result" (EBinop OConcatString (ELoc "result") (EBinop OConcatString (EVar "child") (EAtom (AString "\n")))))) (CAssign "outputs" (EBinop OCons (ELoc "result") (ELoc "outputs")))))))).
 
 Definition heuristics :=
   [
@@ -35,3 +35,49 @@ Definition heuristics :=
     AC [AnnotateCollection; FilterPushdown; ToFilter; ToJoin; ToProj] [[DictIdx "parent"]];
     AC [PushdownCollection; AnnotateCollection; ToFilter; ToJoin; ToProj] [[DictIdx "parent"]]
   ].
+
+Definition row_ty_parents :=
+  TRecord (record_sort [("parent", TString); ("child", TString)]).
+
+Section WithConcreteMaps.
+  Context {width: Z} {word: word.word width} {word_ok: word.ok word}.
+  Notation value := (value (width:=width)).
+
+  Local Open Scope string.
+
+  Instance ctenv : map.map string type := SortedListString.map _.
+  Instance ctenv_ok : map.ok ctenv := SortedListString.ok _.
+
+  Instance clocals : map.map string value := SortedListString.map _.
+  Instance clocals_ok : map.ok clocals := SortedListString.ok _.
+
+  Definition init_Gstore : ctenv :=
+    map.put map.empty "outputs" (TList TString).
+
+  Definition init_Genv : ctenv :=
+    map.put (map.put map.empty
+               "parents_tbl" (TList row_ty_parents))
+      "queries" (TList TString).
+
+  Compute (typecheck init_Gstore init_Genv prog).
+
+  Definition prog_transformed := map (fun heu => apply_optimize_anno (width:=width) (heu prog) init_Gstore init_Genv) heuristics.
+
+  Compute prog_transformed.
+
+  Theorem prog_transformed_sem : forall (store env : clocals),
+      locals_wf init_Gstore store ->
+      locals_wf init_Genv env ->
+      forall prog', In prog' prog_transformed ->
+                    interp_command store env prog' = interp_command store env prog.
+  Proof.
+    unfold prog_transformed, heuristics, apply_optimize_anno; cbn [map]; intros.
+    repeat destruct_In;
+      try eapply transf_sound__preserve_sem;
+      eauto using apply_all_transfs_sound with transf_hints.
+    lazymatch goal with H: In _ [] |- _ => apply in_nil in H; intuition idtac end.
+  Qed.
+End WithConcreteMaps.
+
+Compute program_py prog.
+Compute map program_py prog_transformed.
